Still continuation of  blocking-team proof

ExistentialRules/ChaseSequence/Termination/Linear.lean
@@ -39,19 +39,40 @@ section Rules
       rcases rule_body_len with ⟨a, rule_body_len ⟩
       simp[rule_body_len]
 
+    theorem LinearRule.head_eq {rule : LinearRule sig}: rule.rule.head = [[rule.head.fst, rule.head.snd]] := by
+      unfold LinearRule.head
+      simp
+      have rule_head_len: rule.rule.head.length = 1 := by have det := rule.deterministic; simp only [Rule.isDeterministic, decide_eq_true_iff] at det; exact det
+      have two_atoms: rule.rule.head[0].length = 2 := by have twohead := rule.exactlyTwoHeadAtoms; simp only [Rule.exactlyTwoHeadAtoms] at twohead; exact twohead;
+      revert two_atoms
+      rw[List.length_eq_one_iff] at rule_head_len
+      rcases rule_head_len with ⟨head, rule_head_eq⟩
+      simp[rule_head_eq]
+      --intro lentwo
+      cases head with
+      |nil =>
+        simp
+      |cons a rest =>
+        simp
+        rw[List.length_eq_one_iff]
+        intro rest
+        rcases rest with ⟨x, y ⟩
+        simp[y]
+
    def is_frontier_position_fst (rule: LinearRule sig)  (i: Nat) (i_valid: i < rule.head.fst.terms.length) : Prop :=
       ∃ v, (rule.head.fst.terms[i]'(by exact i_valid)) = VarOrConst.var v ∧ v ∈ rule.rule.frontier
 
-    theorem frontier_pos_body_fst {rule: LinearRule sig} {i: Nat} {i_valid: i < rule.head.fst.terms.length} :
-      is_frontier_position_fst rule i i_valid →
+    theorem frontier_pos_fst_iff_in_body {rule: LinearRule sig} {i: Nat} {i_valid: i < rule.head.fst.terms.length} :
+      is_frontier_position_fst rule i i_valid ↔
       ∃ j , ∃ h: j < rule.body.terms.length, rule.head.fst.terms[i].isVar ∧ rule.head.fst.terms[i] = rule.body.terms[j] := by
       unfold is_frontier_position_fst
-      intro h
+      constructor
+      . intro h
       rcases h with ⟨v, h⟩
-      simp
+        simp only [exists_and_left]
       constructor
       . unfold VarOrConst.isVar
-        simp[h.left]
+          simp only[h.left]
       . rcases rule.rule.frontier_occurs_in_body v h.right with ⟨a, a_body, v_a⟩
         simp only[h]
         simp only[List.mem_iff_getElem] at v_a
@@ -60,15 +81,50 @@ section Rules
         rcases v_a with ⟨c, len, v_a⟩
         exists c, len
         simp[v_a]
+      . intro h
+        rcases h with ⟨j, j_lt, t_var , t_eq⟩
+        have v_ex: ∃ v, rule.head.fst.terms[i] = VarOrConst.var v := by
+          unfold VarOrConst.isVar at t_var
+          cases h: rule.head.fst.terms[i]
+          . simp
+          . simp [h] at t_var
+        rcases v_ex with ⟨v, v_eq⟩
+        exists v
+        simp only[v_eq]
+        unfold Rule.frontier
+        simp only [List.mem_filter, List.any_eq_true, decide_eq_true_eq, true_and]
+        constructor
+        . unfold FunctionFreeConjunction.vars
+          simp only [LinearRule.body_eq, List.flatMap_cons, List.flatMap_nil, List.append_nil]
+          unfold FunctionFreeAtom.variables
+          apply VarOrConst.mem_filterVars_of_var
+          simp only [List.mem_iff_getElem]
+          exists j, j_lt
+          rw[← t_eq]
+          exact v_eq
+        . have rle_head_len: rule.rule.head.length = 1 := by have det := rule.deterministic; simp only [Rule.isDeterministic, decide_eq_true_iff] at det; exact det
+          simp only [List.mem_iff_getElem, rle_head_len]
+          simp only[← List.mem_iff_getElem]
+          unfold FunctionFreeConjunction.vars
+          simp only [LinearRule.head_eq]
+          unfold FunctionFreeAtom.variables
+          simp only [List.getElem_singleton, Nat.lt_one_iff, exists_prop, exists_eq_left,
+            List.mem_flatMap, exists_eq_left', List.mem_cons, List.not_mem_nil, or_false,
+            exists_eq_or_imp]
+          apply Or.inl
+          apply VarOrConst.mem_filterVars_of_var
+          simp only[List.mem_iff_getElem]
+          exists i, i_valid
 
     def is_frontier_position_snd (rule: LinearRule sig)  (i: Nat) (i_valid: i < rule.head.snd.terms.length) : Prop :=
       ∃ v, (rule.head.snd.terms[i]'(by exact i_valid)) = VarOrConst.var v ∧ v ∈ rule.rule.frontier
 
-    theorem frontier_pos_body_snd {rule: LinearRule sig} {i: Nat} {i_valid: i < rule.head.snd.terms.length} :
-      is_frontier_position_snd rule i i_valid →
+    theorem frontier_pos_snd_iff_in_body {rule: LinearRule sig} {i: Nat} {i_valid: i < rule.head.snd.terms.length} :
+      is_frontier_position_snd rule i i_valid ↔
       ∃ j , ∃ h: j < rule.body.terms.length, rule.head.snd.terms[i].isVar ∧ rule.head.snd.terms[i] = rule.body.terms[j] := by
       unfold is_frontier_position_snd
-      intro h
+      constructor
+      . intro h
       rcases h with ⟨v, h⟩
       simp
       constructor
@@ -82,6 +138,41 @@ section Rules
         rcases v_a with ⟨c, len, v_a⟩
         exists c, len
         simp[v_a]
+      . intro h
+        rcases h with ⟨j, j_lt, t_var , t_eq⟩
+        have v_ex: ∃ v, rule.head.snd.terms[i] = VarOrConst.var v := by
+          unfold VarOrConst.isVar at t_var
+          cases h: rule.head.snd.terms[i]
+          . simp
+          . simp [h] at t_var
+        rcases v_ex with ⟨v, v_eq⟩
+        exists v
+        simp only[v_eq]
+        unfold Rule.frontier
+        simp only [List.mem_filter, List.any_eq_true, decide_eq_true_eq, true_and]
+        constructor
+        . unfold FunctionFreeConjunction.vars
+          simp only [LinearRule.body_eq, List.flatMap_cons, List.flatMap_nil, List.append_nil]
+          unfold FunctionFreeAtom.variables
+          apply VarOrConst.mem_filterVars_of_var
+          simp only [List.mem_iff_getElem]
+          exists j, j_lt
+          rw[← t_eq]
+          exact v_eq
+        . have rle_head_len: rule.rule.head.length = 1 := by have det := rule.deterministic; simp only [Rule.isDeterministic, decide_eq_true_iff] at det; exact det
+          simp only [List.mem_iff_getElem, rle_head_len]
+          simp only[← List.mem_iff_getElem]
+          unfold FunctionFreeConjunction.vars
+          simp only [LinearRule.head_eq]
+          unfold FunctionFreeAtom.variables
+          simp only [List.getElem_singleton, Nat.lt_one_iff, exists_prop, exists_eq_left,
+            List.mem_flatMap, exists_eq_left', List.mem_cons, List.not_mem_nil, or_false,
+            exists_eq_or_imp]
+          apply Or.inr
+          apply VarOrConst.mem_filterVars_of_var
+          simp only[List.mem_iff_getElem]
+          exists i, i_valid
+
 
   -- TODO for Lukas: unify this with regular RuleSet at some point
   structure LinearRuleSet (sig : Signature) [DecidableEq sig.P] [DecidableEq sig.C] [DecidableEq sig.V] where
@@ -422,19 +513,21 @@ section SubstitutionsAndTriggers
     rw[ruleApply_eq]
     simp
 
-  theorem ruleApply_frontierPos_fstHead {rule : LinearRule sig} {fact : Fact sig} {i : Nat} (i_valid: i < rule.head.fst.terms.length) (h_frontier : is_frontier_position_fst rule i i_valid):
-     (ruleApplySome: (ruleApply rule fact).isSome) ->
-    ∃ j: Nat, ∃ (j_valid: j < fact.terms.length), ((ruleApply rule fact).get ruleApplySome).fst.terms[i]'(by
-      have trg_some : (PreTrigger.from_rule_and_fact rule fact).isSome := by apply ruleApply.some_implies_PreTrigger_some; exact ruleApplySome
+  theorem ruleApply_fst_term_lenght_eq_rule_head_length {rule:LinearRule sig} {fact: Fact sig} {ruleApply_some: (ruleApply rule fact).isSome}:
+    ((ruleApply rule fact).get ruleApply_some).fst.terms.length = rule.head.fst.terms.length := by
+      have trg_some : (PreTrigger.from_rule_and_fact rule fact).isSome := by apply ruleApply.some_implies_PreTrigger_some; exact ruleApply_some
       rw[Option.isSome_iff_exists] at trg_some
       rcases trg_some with ⟨trg, trg_some⟩
       simp only [ruleApply_eq, trg_some, Option.map_some, Option.get_some]
       simp only [PreTrigger.apply_to_function_free_atom]
       simp only [TermMapping.apply_generalized_atom, List.length_map]
-      exact i_valid
-    ) = fact.terms[j]:= by
+
+  theorem ruleApply_frontierPos_fstHead {rule : LinearRule sig} {fact : Fact sig} {i : Nat} (i_valid: i < rule.head.fst.terms.length) (h_frontier : is_frontier_position_fst rule i i_valid):
+     (ruleApplySome: (ruleApply rule fact).isSome) ->
+    ∃ j: Nat, ∃ (j_valid: j < fact.terms.length), ((ruleApply rule fact).get ruleApplySome).fst.terms[i]'(by
+      rw[ruleApply_fst_term_lenght_eq_rule_head_length]; exact i_valid) = fact.terms[j]:= by
     intro ruleApplyIsSome
-    rcases frontier_pos_body_fst h_frontier with ⟨j, j_valid, h_frontier'⟩
+    rcases (frontier_pos_fst_iff_in_body).mp h_frontier with ⟨j, j_valid, h_frontier'⟩
 
     have trg_some : (PreTrigger.from_rule_and_fact rule fact).isSome := by apply ruleApply.some_implies_PreTrigger_some; exact ruleApplyIsSome
     rw[Option.isSome_iff_exists] at trg_some
@@ -471,7 +564,7 @@ section SubstitutionsAndTriggers
       exact i_valid
     ) = fact.terms[j]:= by
     intro ruleApplyIsSome
-    rcases frontier_pos_body_snd h_frontier with ⟨j, j_valid, h_frontier'⟩
+    rcases (frontier_pos_snd_iff_in_body).mp h_frontier with ⟨j, j_valid, h_frontier'⟩
 
     have trg_some : (PreTrigger.from_rule_and_fact rule fact).isSome := by apply ruleApply.some_implies_PreTrigger_some; exact ruleApplyIsSome
     rw[Option.isSome_iff_exists] at trg_some
@@ -495,6 +588,38 @@ section SubstitutionsAndTriggers
     rw [PreTrigger.apply_to_var_or_const_frontier_var _ _ _ (by rw [← trg_eq]; exact v_front)]
     rw [← trg_eq]
     rfl
+
+  theorem ruleApply_non_frontier_Var_fst_head {rule: LinearRule sig} {fact: Fact sig} {i : Nat} (i_valid: i < rule.head.fst.terms.length) (no_frontier : ¬ is_frontier_position_fst rule i i_valid):
+     (ruleApplySome: (ruleApply rule fact).isSome) -> (t_isVar:∃ v, rule.head.fst.terms[i] = VarOrConst.var v) ->
+     ((ruleApply rule fact).get ruleApplySome).fst.terms[i]'(by rw[ruleApply_fst_term_lenght_eq_rule_head_length]; exact i_valid) ∉ fact.terms := by
+    intro ruleApplySome t_isVar
+    simp[ruleApply_eq]
+    unfold PreTrigger.apply_to_function_free_atom
+    unfold TermMapping.apply_generalized_atom
+    simp only [List.getElem_map]
+
+    unfold is_frontier_position_fst at no_frontier
+    simp[not_exists] at no_frontier
+    rcases t_isVar with ⟨v, v_eq⟩
+    simp[v_eq] at no_frontier
+
+    have trg_some : (PreTrigger.from_rule_and_fact rule fact).isSome := by apply ruleApply.some_implies_PreTrigger_some; exact ruleApplySome
+    rw[Option.isSome_iff_exists] at trg_some
+    rcases trg_some with ⟨trg, trg_some⟩
+    have trg_some' := trg_some
+    unfold PreTrigger.from_rule_and_fact at trg_some
+    simp[Option.map_eq_some_iff] at trg_some
+    rcases trg_some with ⟨sub, sub_def, trg_eq⟩
+    --rw[trg_eq] at no_frontier
+    --have sub_apply: sub.apply_function_free_atom rule.body = fact := by
+    --  rw[GroundSubstitution.apply_function_free_atom_from_atom_and_fact]
+    --  exact sub_def
+    simp only [trg_some', Option.get_some]
+    rw[v_eq]
+    rw[PreTrigger.apply_to_var_or_const_non_frontier_var trg 0 v (by sorry)]
+    unfold PreTrigger.functional_term_for_var
+
+    sorry
 
 end SubstitutionsAndTriggers
 
@@ -664,6 +789,19 @@ section TriggersAndChaseDerivation
             unfold PreTrigger.apply_to_function_free_atom PreTrigger.apply_to_var_or_const TermMapping.apply_generalized_atom;
             simp;
 
+    theorem trg_apply_labelling_fst_terms_len {fs: FactSet sig} {pi: LinearRuleTrigger fs rs} :
+          pi.rule.val.head.fst.terms.length = (labelling_of_apply pi).fst.terms.length := by
+        rw[GeneralizedAtom.arity_ok]
+        simp only[trg_apply_labelling_fst_predicate_eq]
+        rw[← GeneralizedAtom.arity_ok]
+
+    theorem trg_apply_labelling_snd_terms_len {fs: FactSet sig} {pi: LinearRuleTrigger fs rs} :
+          pi.rule.val.head.snd.terms.length = (labelling_of_apply pi).snd.terms.length := by
+        rw[GeneralizedAtom.arity_ok]
+        simp only[trg_apply_labelling_snd_predicate_eq]
+        rw[← GeneralizedAtom.arity_ok]
+
+
     def appears_in_forest {fs: FactSet sig} (pi: LinearRuleTrigger fs rs) (g: Forest fs rs): Prop := pi.addr.val ∈ g.f
 
     -- TODO for Laila: If you want, you can instantiate the Membership typeclass for triggers and forests to be able to write: pi ∈ g and define this to be pi.appears_in_forest g
@@ -699,26 +837,65 @@ section TriggersAndChaseDerivation
     structure Conditions {fs: FactSet sig} {g : Forest fs rs} (g_sub: g.subforest_of (oblivious_chase fs rs)) (b1 b2: forest_Address g) (pi: forest_Trigger g) where
       b1_label := Option.get (labellingFunction b1.val) (by apply forest_addr_label_some; exact g_sub)
       b2_label:= Option.get (labellingFunction b2.val) (by apply forest_addr_label_some; exact g_sub)
+      b1_label_eq : b1_label = Option.get (labellingFunction b1.val) (by apply forest_addr_label_some; exact g_sub) := by rfl
+      b2_label_eq : b2_label = Option.get (labellingFunction b2.val) (by apply forest_addr_label_some; exact g_sub) := by rfl
       --rule := pi.val.rule.val
       first : (b1_label.predicate = (labelling_of_apply pi.val).fst.predicate)
         ∧ (b2_label.predicate = (labelling_of_apply pi.val).snd.predicate)
-      second :
-        (∀ j, (lt_fst: j < pi.val.rule.val.head.fst.terms.length) -> is_frontier_position_fst pi.val.rule.val j lt_fst ->
-          (labelling_of_apply pi.val).fst.terms[j]'(by rw[GeneralizedAtom.arity_ok, ← trg_apply_labelling_fst_predicate_eq, ← GeneralizedAtom.arity_ok]; simp[lt_fst]) = b1_label.terms[j]'(by rw[GeneralizedAtom.arity_ok, first.left, ← trg_apply_labelling_fst_predicate_eq, ← GeneralizedAtom.arity_ok]; simp[lt_fst]))
-        ∧ (∀ j, (lt_snd: j < pi.val.rule.val.head.snd.terms.length) -> is_frontier_position_snd pi.val.rule.val j lt_snd ->
-          (labelling_of_apply pi.val).snd.terms[j]'(by rw[GeneralizedAtom.arity_ok, ← trg_apply_labelling_snd_predicate_eq, ← GeneralizedAtom.arity_ok]; simp[lt_snd]) = b2_label.terms[j]'(by rw[GeneralizedAtom.arity_ok, first.right, ← trg_apply_labelling_snd_predicate_eq, ← GeneralizedAtom.arity_ok]; simp[lt_snd]))
+      second : --note that this slightly differs from the original paper as constant were neglected there
+        (∀ j, (lt_fst: j < pi.val.rule.val.head.fst.terms.length) -> (is_frontier_position_fst pi.val.rule.val j lt_fst) ∨ (∃ c, pi.val.rule.val.head.fst.terms[j] = VarOrConst.const c) ->
+          (labelling_of_apply pi.val).fst.terms[j]'(by rw[← trg_apply_labelling_fst_terms_len]; exact lt_fst) = b1_label.terms[j]'(by rw[GeneralizedAtom.arity_ok, first.left, ← trg_apply_labelling_fst_predicate_eq, ← GeneralizedAtom.arity_ok]; simp[lt_fst]))
+        ∧ (∀ j, (lt_snd: j < pi.val.rule.val.head.snd.terms.length) -> (is_frontier_position_snd pi.val.rule.val j lt_snd) ∨ (∃ c, pi.val.rule.val.head.snd.terms[j] = VarOrConst.const c) ->
+          (labelling_of_apply pi.val).snd.terms[j]'(by rw[← trg_apply_labelling_snd_terms_len]; exact lt_snd) = b2_label.terms[j]'(by rw[GeneralizedAtom.arity_ok, first.right, ← trg_apply_labelling_snd_predicate_eq, ← GeneralizedAtom.arity_ok]; simp[lt_snd]))
       third : (∀ i j:Nat, (labelling_of_apply pi.val).fst.terms[i]? = (labelling_of_apply pi.val).fst.terms[j]? -> b1_label.terms[i]? = b1_label.terms[j]?) --funktioniert das mit dem indizieren mit [.]? so?
         ∧ (∀ i j:Nat, (labelling_of_apply pi.val).fst.terms[i]? = (labelling_of_apply pi.val).snd.terms[j]? -> b1_label.terms[i]? = b2_label.terms[j]?)
         ∧ (∀ i j:Nat, (labelling_of_apply pi.val).snd.terms[i]? = (labelling_of_apply pi.val).snd.terms[j]? -> b2_label.terms[i]? = b2_label.terms[j]?)
 
-    theorem Conditions.b1_label_eq {fs: FactSet sig} {g : Forest fs rs}{g_sub: g.subforest_of (oblivious_chase fs rs)} {b1 b2: forest_Address g} {pi: forest_Trigger g} {cond : Conditions g_sub b1 b2 pi} :
-    cond.b1_label =  Option.get (labellingFunction b1.val) (by apply forest_addr_label_some; exact g_sub) := by simp only[Conditions, Conditions.b1_label]; rfl; sorry
+    theorem b1_label_terms_idxOf_eq {fs: FactSet sig} {g : Forest fs rs} {g_sub: g.subforest_of (oblivious_chase fs rs)} {b1 b2: forest_Address g} {pi: forest_Trigger g} {cond: Conditions g_sub b1 b2 pi}:
+        ∀i, (i_lt:  i < pi.val.labelling_of_apply.fst.terms.length) -> cond.b1_label.terms[List.idxOf pi.val.labelling_of_apply.fst.terms[i] pi.val.labelling_of_apply.fst.terms]'
+          (by rw[GeneralizedAtom.arity_ok, cond.first.left, ← GeneralizedAtom.arity_ok]; simp[List.idxOf_lt_length_iff])
+        = cond.b1_label.terms[i]'(by rw[GeneralizedAtom.arity_ok, cond.first.left, ← GeneralizedAtom.arity_ok]; exact i_lt) := by
+      intro i i_lt
+      by_cases i_eq: i = List.idxOf pi.val.labelling_of_apply.fst.terms[i] pi.val.labelling_of_apply.fst.terms
+      . simp[← i_eq]
+      . have mem_l: pi.val.labelling_of_apply.fst.terms[i] ∈ pi.val.labelling_of_apply.fst.terms := by
+          simp[List.mem_iff_getElem]
+          exists i, i_lt
+        have idxLt: List.idxOf pi.val.labelling_of_apply.fst.terms[i] pi.val.labelling_of_apply.fst.terms < pi.val.labelling_of_apply.fst.terms.length:= by
+          simp[List.idxOf_lt_length_iff]
+        let trd:= cond.third.left
+        rw[← Option.some_inj]
+        simp[← List.getElem?_eq_getElem]
+        apply trd
+        rw[List.getElem?_eq_getElem idxLt];
+        rw[List.getElem_idxOf_of_mem mem_l]
+        simp
+
+    theorem b2_label_terms_idxOf_eq {fs: FactSet sig} {g : Forest fs rs} {g_sub: g.subforest_of (oblivious_chase fs rs)} {b1 b2: forest_Address g} {pi: forest_Trigger g} {cond: Conditions g_sub b1 b2 pi}:
+        ∀i, (i_lt:  i < pi.val.labelling_of_apply.snd.terms.length) -> cond.b2_label.terms[List.idxOf pi.val.labelling_of_apply.snd.terms[i] pi.val.labelling_of_apply.snd.terms]'
+          (by rw[GeneralizedAtom.arity_ok, cond.first.right, ← GeneralizedAtom.arity_ok]; simp[List.idxOf_lt_length_iff])
+        = cond.b2_label.terms[i]'(by rw[GeneralizedAtom.arity_ok, cond.first.right, ← GeneralizedAtom.arity_ok]; exact i_lt) := by
+      intro i i_lt
+      by_cases i_eq: i = List.idxOf pi.val.labelling_of_apply.snd.terms[i] pi.val.labelling_of_apply.snd.terms
+      . simp[← i_eq]
+      . have mem_l: pi.val.labelling_of_apply.snd.terms[i] ∈ pi.val.labelling_of_apply.snd.terms := by
+          simp[List.mem_iff_getElem]
+          exists i, i_lt
+        have idxLt: List.idxOf pi.val.labelling_of_apply.snd.terms[i] pi.val.labelling_of_apply.snd.terms < pi.val.labelling_of_apply.snd.terms.length:= by
+          simp[List.idxOf_lt_length_iff]
+        let trd:= cond.third.right.right
+        rw[← Option.some_inj]
+        simp[← List.getElem?_eq_getElem]
+        apply trd
+        rw[List.getElem?_eq_getElem idxLt];
+        rw[List.getElem_idxOf_of_mem mem_l]
+        simp
 
     theorem blockingTeam.iff {fs: FactSet sig} {g : Forest fs rs} {g_sub: g.subforest_of (oblivious_chase fs rs)} {b1 b2: forest_Address g} {pi: forest_Trigger g} :
       blockingTeam g_sub b1 b2 pi ↔ ∃ cond : Conditions g_sub b1 b2 pi, True := by
         unfold blockingTeam
-
         constructor
+        -- direction →
         . unfold GroundTermMapping.applyFact TermMapping.apply_generalized_atom--GroundTermMapping.isIdOnConstants
           intro a
           rcases a with ⟨h, a ⟩
@@ -730,20 +907,21 @@ section TriggersAndChaseDerivation
             . rw[← a.right.left]
             . rw[ ← a.right.right.left]
           have snd_cond:
-           (∀ j, (lt_fst: j < pi.val.rule.val.head.fst.terms.length) -> is_frontier_position_fst pi.val.rule.val j lt_fst ->
-           (labelling_of_apply pi.val).fst.terms[j]'(by rw[GeneralizedAtom.arity_ok, ← trg_apply_labelling_fst_predicate_eq, ← GeneralizedAtom.arity_ok]; simp[lt_fst])
+           (∀ j, (lt_fst: j < pi.val.rule.val.head.fst.terms.length) -> (is_frontier_position_fst pi.val.rule.val j lt_fst) ∨ (∃ c, pi.val.rule.val.head.fst.terms[j] = VarOrConst.const c) ->
+           (labelling_of_apply pi.val).fst.terms[j]'(by rw[← trg_apply_labelling_fst_terms_len]; exact lt_fst)
             = b1_label.terms[j]'(by rw[GeneralizedAtom.arity_ok, fst_cond.left,  ← trg_apply_labelling_fst_predicate_eq, ← GeneralizedAtom.arity_ok]; simp[lt_fst]))
             ∧
-            (∀ j, (lt_snd: j < pi.val.rule.val.head.snd.terms.length) -> is_frontier_position_snd pi.val.rule.val j lt_snd ->
-           (labelling_of_apply pi.val).snd.terms[j]'(by rw[GeneralizedAtom.arity_ok, ← trg_apply_labelling_snd_predicate_eq, ← GeneralizedAtom.arity_ok]; simp[lt_snd])
+            (∀ j, (lt_snd: j < pi.val.rule.val.head.snd.terms.length) -> (is_frontier_position_snd pi.val.rule.val j lt_snd) ∨ (∃ c, pi.val.rule.val.head.snd.terms[j] = VarOrConst.const c) ->
+           (labelling_of_apply pi.val).snd.terms[j]'(by rw[← trg_apply_labelling_snd_terms_len]; exact lt_snd)
            = b2_label.terms[j]'(by rw[GeneralizedAtom.arity_ok, fst_cond.right,  ← trg_apply_labelling_snd_predicate_eq, ← GeneralizedAtom.arity_ok]; simp[lt_snd])):= by
            constructor
            .intro j j_valid
             unfold b1_label
-            intro j_frontier_pos
-            simp[← a.right.left]
+            simp only [or_imp, forall_exists_index]
+            constructor
+            . intro j_frontier_pos
+              simp only [← a.right.left, List.getElem_map]
             unfold labelling_of_apply
-            simp
             rcases ruleApply_frontierPos_fstHead (rule := pi.val.rule.val) (fact := (Option.get (labellingFunction pi.val.addr.val) pi.val.addr.property)) (i := j) j_valid j_frontier_pos (by
               simp[ruleApply_of_trigger_labelling_is_some]) with ⟨k, k_valid, eq⟩
             rw [eq]
@@ -751,12 +929,30 @@ section TriggersAndChaseDerivation
             rw [GeneralizedAtom.mk.injEq] at a_left
             conv => left; arg 1; rw [← a_left.right]
             rw [List.getElem_map]
+            . intro c c_eq
+              simp only [← a.right.left, List.getElem_map]
+
+              have hc_id : h (GroundTerm.const c) = (GroundTerm.const c) := by
+                unfold GroundTerm.const
+                let h_const_id:= a.right.right.right
+                unfold GroundTermMapping.isIdOnConstants at h_const_id
+                rw[h_const_id ⟨FiniteTree.leaf c, GroundTerm.const._proof_1 c⟩ ]
+
+              unfold labelling_of_apply
+              simp only [ruleApply_eq, Option.get_map]
+              unfold PreTrigger.apply_to_function_free_atom
+              unfold TermMapping.apply_generalized_atom
+              rw[List.getElem_map]
+              rw[c_eq]
+              rw[PreTrigger.apply_to_var_or_const_for_const]
+              simp[hc_id]
            .intro j j_valid
             unfold b2_label
-            intro j_frontier_pos
-            simp[← a.right.right.left]
+            simp only [or_imp, forall_exists_index]
+            constructor
+            . intro j_frontier_pos
+              simp only[← a.right.right.left, List.getElem_map]
             unfold labelling_of_apply
-            simp
             rcases ruleApply_frontierPos_sndHead (rule := pi.val.rule.val) (fact := (Option.get (labellingFunction pi.val.addr.val) pi.val.addr.property)) (i := j) j_valid j_frontier_pos (by
               simp[ruleApply_of_trigger_labelling_is_some]) with ⟨k, k_valid, eq⟩
             rw [eq]
@@ -764,6 +960,24 @@ section TriggersAndChaseDerivation
             rw [GeneralizedAtom.mk.injEq] at a_left
             conv => left; arg 1; rw [← a_left.right]
             rw [List.getElem_map]
+            . intro c c_eq
+              simp only [← a.right.right.left, List.getElem_map]
+
+              have hc_id : h (GroundTerm.const c) = (GroundTerm.const c) := by
+                unfold GroundTerm.const
+                let h_const_id:= a.right.right.right
+                unfold GroundTermMapping.isIdOnConstants at h_const_id
+                rw[h_const_id ⟨FiniteTree.leaf c, GroundTerm.const._proof_1 c⟩ ]
+
+              unfold labelling_of_apply
+              simp only [ruleApply_eq, Option.get_map]
+              unfold PreTrigger.apply_to_function_free_atom
+              unfold TermMapping.apply_generalized_atom
+              rw[List.getElem_map]
+              rw[c_eq]
+              rw[PreTrigger.apply_to_var_or_const_for_const]
+              simp[hc_id]
+
           have trd_cond:
           (∀ i j:Nat, (labelling_of_apply pi.val).fst.terms[i]? = (labelling_of_apply pi.val).fst.terms[j]? -> b1_label.terms[i]? = b1_label.terms[j]?)
           ∧ (∀ i j:Nat, (labelling_of_apply pi.val).fst.terms[i]? = (labelling_of_apply pi.val).snd.terms[j]? -> b1_label.terms[i]? = b2_label.terms[j]?)
@@ -779,14 +993,213 @@ section TriggersAndChaseDerivation
               . intro i j hyp
                 simp[hyp]
           exists {first := fst_cond , second:= snd_cond, third:= trd_cond}
+        -- direction ←
         . intro a
           rcases a with ⟨cond, a⟩
           let fst := cond.first
           let snd := cond.second
           let trd := cond.third
+
+          --have b1_label_terms_len: cond.b1_label.terms.length = pi.val.rule.val.head.fst.terms.length := by sorry
           --unfold Conditions.b1_label at fst
           unfold GroundTermMapping.applyFact TermMapping.apply_generalized_atom
+          let h: GroundTermMapping sig := fun t =>
+            if tInFst: t ∈ (labelling_of_apply pi.val).fst.terms
+            then cond.b1_label.terms[(labelling_of_apply pi.val).fst.terms.idxOf t]'(by
+              rw[Atom_pred_eq_implies_eq_term_length cond.first.left];
+              rw[List.idxOf_lt_length_iff]; exact tInFst)
+            else if tInSnd: t ∈ (labelling_of_apply pi.val).snd.terms
+              then cond.b2_label.terms[(labelling_of_apply pi.val).snd.terms.idxOf t]'(by
+                rw[Atom_pred_eq_implies_eq_term_length cond.first.right];
+                rw[List.idxOf_lt_length_iff]; exact tInSnd)
+              else t
+          exists h
+          constructor
+          -- show h(⟨u⟩) = ⟨u⟩
+          . rw[GeneralizedAtom.mk.injEq]
+            simp only[true_and]
+            rw[List.map_eq_iff]
+            intro i
+            unfold Option.map
+            by_cases i_len: i <  ((labellingFunction pi.val.addr.val).get pi.val.addr.property).terms.length
+            . simp[i_len]
+              simp[h]
+              by_cases mem_labelling_of_apply_fst: ((labellingFunction pi.val.addr.val).get pi.val.addr.property).terms[i] ∈ pi.val.labelling_of_apply.fst.terms
+              -- ⟨u⟩_i occurs in ⟨up1⟩  (in pi.val.labelling_of_apply.fst.terms )
+              . simp only[mem_labelling_of_apply_fst]
+                simp only[List.mem_iff_getElem] at mem_labelling_of_apply_fst
+                rcases mem_labelling_of_apply_fst with ⟨idx, idx_lt, t_eq⟩
+                simp only [← t_eq, ↓reduceDIte]
+                have idx_lt_rulehead: idx < pi.val.rule.val.head.fst.terms.length := by rw[trg_apply_labelling_fst_terms_len]; exact idx_lt
+                by_cases inFrontier: is_frontier_position_fst pi.val.rule.val idx idx_lt_rulehead
+                . let idx_of:= List.idxOf pi.val.labelling_of_apply.fst.terms[idx] pi.val.labelling_of_apply.fst.terms
+                  have mem_l: pi.val.labelling_of_apply.fst.terms[idx] ∈ pi.val.labelling_of_apply.fst.terms := by
+                    simp only[List.mem_iff_getElem]
+                    exists idx, idx_lt
+                  rw[b1_label_terms_idxOf_eq]
+                  simp[snd.left idx idx_lt_rulehead (Or.inl inFrontier)]
+
+                -- term not in frontier -> this may be hard to show
+                . sorry
+              --term not in labelling_of_apply.fst.terms
+              . simp only [mem_labelling_of_apply_fst, ↓reduceDIte, right_eq_dite_iff]
+                intro mem_labelling_of_apply_snd
+                simp only[List.mem_iff_getElem] at mem_labelling_of_apply_snd
+                rcases mem_labelling_of_apply_snd with ⟨idx, idx_lt, t_eq⟩
+                simp only [← t_eq]
+                have idx_lt_rulehead: idx < pi.val.rule.val.head.snd.terms.length := by rw[trg_apply_labelling_snd_terms_len]; exact idx_lt
+                by_cases inFrontier: is_frontier_position_snd pi.val.rule.val idx idx_lt_rulehead
+                . let idx_of:= List.idxOf pi.val.labelling_of_apply.snd.terms[idx] pi.val.labelling_of_apply.snd.terms
+                  have mem_l: pi.val.labelling_of_apply.snd.terms[idx] ∈ pi.val.labelling_of_apply.snd.terms := by
+                    simp only[List.mem_iff_getElem]
+                    exists idx, idx_lt
+                  rw[b2_label_terms_idxOf_eq]
+                  simp[snd.right idx idx_lt_rulehead (Or.inl inFrontier)]
+
+                -- term not in frontier -> this may be hard to show
+                . sorry
+
+            . simp [i_len]
+          . constructor
+            --shows h(⟨up_1⟩) = ⟨v_1⟩  i.e. h (pi.val.labelling_of_apply.fst) = (labellingFunction b1.val).get ...
+            . rw[GeneralizedAtom.mk.injEq]
+              rw[← fst.left]
+              simp only [cond.b1_label_eq, true_and]
+              rw[List.map_eq_iff]
+              intro i
+              unfold Option.map
+              by_cases i_len: i <  pi.val.labelling_of_apply.fst.terms.length
+              . simp[i_len] --, List.getElem?_eq_some_iff];
+                have i_lt : i < ((labellingFunction b1.val).get (by apply forest_addr_label_some; exact g_sub)).terms.length := by
+                  rw[← cond.b1_label_eq]
+                  rw[Atom_pred_eq_implies_eq_term_length fst.left]
+                  exact i_len
+                simp only [List.getElem_mem, ↓reduceDIte, h, List.getElem?_eq_some_iff]
+                exists i_lt
+                rw[b1_label_terms_idxOf_eq]
+                simp only[cond.b1_label_eq]
+              . simp only [i_len, not_false_eq_true, getElem?_neg, getElem?_eq_none_iff, Nat.not_lt]
+                rw[← cond.b1_label_eq]
+                rw[Atom_pred_eq_implies_eq_term_length fst.left]
+                rw[← Nat.not_lt]
+                exact i_len
+            . constructor
+              --shows h(⟨up_2⟩) = ⟨v_2⟩  i.e. h (pi.val.labelling_of_apply.snd) = (labellingFunction b2.val).get ...
+              . rw[GeneralizedAtom.mk.injEq]
+                rw[← fst.right]
+                simp only [cond.b2_label_eq, true_and]
+                rw[List.map_eq_iff]
+                intro i
+                unfold Option.map
+                by_cases i_len: i <  pi.val.labelling_of_apply.snd.terms.length
+                . simp only [i_len, getElem?_pos]
+                  have i_lt : i < ((labellingFunction b2.val).get (by apply forest_addr_label_some; exact g_sub)).terms.length := by
+                    rw[← cond.b2_label_eq]
+                    rw[Atom_pred_eq_implies_eq_term_length fst.right]
+                    exact i_len
+                  simp only [List.getElem_mem, ↓reduceDIte, h, List.getElem?_eq_some_iff]
+                  exists i_lt
+                  by_cases term_mem_labelling_of_apply_fst: pi.val.labelling_of_apply.snd.terms[i] ∈ pi.val.labelling_of_apply.fst.terms
+                  . simp only [term_mem_labelling_of_apply_fst, ↓reduceDIte]
+                    have idxLt: List.idxOf pi.val.labelling_of_apply.snd.terms[i] pi.val.labelling_of_apply.fst.terms < pi.val.labelling_of_apply.fst.terms.length:= by
+                        simp[List.idxOf_lt_length_iff]
+                        exact term_mem_labelling_of_apply_fst
+                    let trd:= cond.third.right.left
+                    rw[← Option.some_inj]
+                    simp only[← List.getElem?_eq_getElem]
+                    rw[← cond.b2_label_eq, eq_comm]
+                    apply trd
+                    rw[List.getElem?_eq_getElem idxLt]
+                    rw[List.getElem_idxOf_of_mem term_mem_labelling_of_apply_fst]
+                    simp
+                  . simp only[term_mem_labelling_of_apply_fst]
+                    rw[b2_label_terms_idxOf_eq]
+                    simp[cond.b2_label_eq]
+                . simp only [i_len, not_false_eq_true, getElem?_neg, getElem?_eq_none_iff]
+                  rw[← cond.b2_label_eq]
+                  rw[Atom_pred_eq_implies_eq_term_length fst.right]
+                  exact i_len
+
+              -- shows h.isIdOnConstants
+              . unfold GroundTermMapping.isIdOnConstants
+                intro t
+                by_cases e_def: ∃ c, t = GroundTerm.const c
+                . unfold GroundTerm.const at e_def
+                  rcases e_def with ⟨c, c_def⟩
+                  simp[c_def]
+                  rw[← c_def]
+                  unfold h
+                  by_cases mem_apply_label: t ∈ pi.val.labelling_of_apply.fst.terms
+                  -- t occurs in pi.val.labelling_of_apply
+                  -- Baisically t can either be in a frontier position, then h(t) = t by the snd.condition,
+                  -- or t is not frontier, then
+                  -- either c was a Constant already in the rule or it was an ex. Vatiable and therefore will be mapped to a null, not a constant which gives a contradiction
+                  . simp[mem_apply_label]
+                    have listIdx_lt: List.idxOf t pi.val.labelling_of_apply.fst.terms < pi.val.labelling_of_apply.fst.terms.length := by
+                      simp[List.idxOf_lt_length_iff]
+                      exact mem_apply_label
+                    have listIdx_lt_rule_head: List.idxOf t pi.val.labelling_of_apply.fst.terms < pi.val.rule.val.head.fst.terms.length := by
+                      rw[trg_apply_labelling_fst_terms_len]
+                      simp[List.idxOf_lt_length_iff]
+                      exact mem_apply_label
+                    simp[List.mem_iff_getElem] at mem_apply_label
+                    rcases mem_apply_label with ⟨i, i_lt, t_eq⟩
+                    have i_lt_rulehead: i < pi.val.rule.val.head.fst.terms.length := by rw[GeneralizedAtom.arity_ok, trg_apply_labelling_fst_predicate_eq, ← GeneralizedAtom.arity_ok]; exact i_lt
+                    --rw[← snd.left]
+                    --simp[List.getElem_idxOf_of_mem mem_apply_label]
+                    --rw[trg_apply_labelling_fst_terms_len]
+                    --exact listIdx_lt
+                   -- false_or_by_contra
+                   -- rename_i aha
+
+                    --simp[List.getElem_idxOf_of_mem mem_apply_label]
+                    by_cases inFrontier: is_frontier_position_fst pi.val.rule.val (List.idxOf t pi.val.labelling_of_apply.fst.terms) listIdx_lt_rule_head
+                     -- term is in frontier
+                    . let idx_of:= List.idxOf pi.val.labelling_of_apply.fst.terms[i] pi.val.labelling_of_apply.fst.terms
+                      have mem_l: pi.val.labelling_of_apply.fst.terms[i] ∈ pi.val.labelling_of_apply.fst.terms := by
+                        simp[List.mem_iff_getElem]
+                        exists i, i_lt
+
+                      rw[← snd.left (List.idxOf t pi.val.labelling_of_apply.fst.terms) listIdx_lt_rule_head (Or.inl inFrontier)]
+                      rw[List.getElem_idxOf_of_mem mem_apply_label]
+
+                      -- term not in frontier
+                    . by_cases constant_in_rule: ∃ c, pi.val.rule.val.head.fst.terms[(List.idxOf t pi.val.labelling_of_apply.fst.terms)] = VarOrConst.const c
+                      . rw[← snd.left (List.idxOf t pi.val.labelling_of_apply.fst.terms) listIdx_lt_rule_head (Or.inr constant_in_rule)]
+                        rw[List.getElem_idxOf_of_mem mem_apply_label]
+                      . -- term is neither in frontier nor constant -> must be a non-frontier-variable; should lead to contradiction
+                        simp only[cond.b1_label_eq]
+                        --simp[List.getElem_map]
+                        unfold labellingFunction
+                        --rw[← List.getElem_map]
+                        simp[ruleApply_eq]
+                        --simp[Option.get]
+                        unfold PreTrigger.apply_to_function_free_atom
+
+                        have t_is_var: ∃ v, pi.val.rule.val.head.fst.terms[List.idxOf t pi.val.labelling_of_apply.fst.terms] = VarOrConst.var v := by sorry
+
+                        rcases t_is_var with ⟨v, v_eq⟩
+
+                        unfold is_frontier_position_fst at inFrontier
+                        rw[not_exists] at inFrontier
+                        simp at inFrontier
+                        simp[v_eq] at inFrontier
+
+
+
+                        rw[PreTrigger.apply_to_var_or_const_non_frontier_var]
+
+                        sorry
+
+                  . simp[mem_apply_label]
+                    intro t_in_snd_label
+
+                    sorry
+                . unfold GroundTerm.const at e_def
+                  simp[not_exists] at e_def
+                  simp
           --simp[List.idxOf]
+          /-
           let h: GroundTermMapping sig := fun t =>
             match t with
               | .const c => t
@@ -841,7 +1254,7 @@ section TriggersAndChaseDerivation
                 . unfold GroundTerm.const at e_def
                   simp[not_exists] at e_def
                   simp
-
+        -/
           /- fun h : GroundTermMapping sig := fun t => -/
           /-   if t ∈ .. then t else  -/
           /-     if t ∈ ....fst then b1_label.terms[...fst.indexOf t] -/
